WIP: Coe-stuff 🍊

RuleSystem/Rules/Capture.lean
@@ -19,4 +19,27 @@ def captureOnTaggedFromSingle {n : ℕ} (rule : Rule n) := captureOnTagged {rule
 -- The corresponding subtype
 def CaptureOnTagged {n : ℕ} (rules : Rules n) := Subtype (· ∈ captureOnTagged rules)
 
+-- TODO: Naming
+def captureEmbed {n : ℕ} (rule : Rule n) := rule.captureFromSingle |> Instances.castSucc
+-- def captureEmbed {n : ℕ} (rule : Rule n) : Finset (@Instances.notContainingLast n)
+--   := rule.captureFromSingle |> Instances.castSucc
+
+def embedCapture {n : ℕ} (rule : Rule n) := rule.castSucc.captureFromSingle
+
+instance coeDepCaptureEmbedNotContainingLast {n : ℕ} (rule : Rule n) (inst : rule.captureEmbed)
+  : CoeDep rule.captureEmbed inst (@Instances.notContainingLast n) where
+    coe := by
+      exists inst
+      simp [Instances.notContainingLast]
+      intro last_mem_inst_tags
+      have := inst.property
+      simp only [Rule.captureEmbed, Rule.captureFromSingle, Instances.castSucc, Instance.castSuccEmbedding, capture, applyTo, appliesTo] at this
+      cases rule_eq : rule <;> (
+        simp [rule_eq] at this
+        obtain ⟨_, _, inst'_castSucc_eq_inst⟩ := this
+        simp [Instance.castSucc, Finset.castSucc, Fin.castSuccEmb, Fin.castAddEmb, Fin.castLEEmb] at inst'_castSucc_eq_inst
+        simp [← inst'_castSucc_eq_inst] at last_mem_inst_tags
+        obtain ⟨_, _, castLE_eq_last⟩ := last_mem_inst_tags
+        exact Fin.false_of_castLE_eq_last castLE_eq_last)
+
 end Rule
