RuleSystem/Rules/Theorems/Embeddings/PositiveWip.lean
@@ -1,4 +1,5 @@
 import RuleSystem.Rules.Theorems.Embeddings.Positive
+import RuleSystem.Rules.Wip
 
 -- TODO: Minimize imports
 
@@ -6,29 +7,15 @@ namespace Rule
 
 namespace Positive
 
--- TODO: These defs should be somewhere else
-
--- TODO: Naming
-def captureEmbed {n : ℕ} (rule : Positive n) := rule.val.captureFromSingle |> Instances.castSucc
-
--- TODO: Move to Instances.lean
--- TODO: Naming
-def insertLast' {n : ℕ} (inst : Instance (n + 1)) : Instance (n + 1) := ⟨inst.tags ∪ {Fin.last _}⟩
-
--- TODO: Fix these, move them to the correct place
--- def insertLast'_embedding {n : ℕ} : Finset (Instance (n + 1)) ↪ Finset (Instance (n + 1)) :=
---   ⟨insertLast', by simp [Function.Injective, insertLast']⟩
-
--- def insertLast {n : ℕ} (instances : Instances n) := instances.map insertLast'_embedding
-
 -- 🔮 (EP-3)
 -- TODO: Naming
 -- TODO: Fix the theorem statement, what we want to do is basically
 --          `captureEmbed ∪ captureEmbed.insertLast = embedCapture`
+-- TODO: Use `Finset.disjUnion` here
 theorem ep_3
     {n : ℕ}
     {rule : Positive n}
-  : (rule.val.captureFromSingle |> Instances.castSucc) = rule.val.castSucc.captureFromSingle := by
+  : rule.val.captureEmbed ∪ (Instances.insertLast' rule.val.captureEmbed) = rule.val.embedCapture := by
     sorry
 
 end Positive
