RuleSystem/Rules/Wip.lean
@@ -1,0 +1,23 @@
+import RuleSystem.Rules.Theorems.Advanced
+
+namespace Rule
+
+
+-- TODO: Finish this 🍊
+-- application type mismatch
+--   Instances.insertLast' (↑rule).captureEmbed
+-- argument
+--   (↑rule).captureEmbed
+-- has type
+--   Instances (n + 1) : Type
+-- but is expected to have type
+--   Finset { x // x ∈ Instances.notContainingLast } : Type
+
+-- This is probably wrong / not what we want
+-- instance CoeDepCaptureEmbedNotContainingLast {n : ℕ} (rule : Rule n)
+--   : CoeDep (Instances (n + 1)) rule.captureEmbed (Finset (@Instances.notContainingLast n)) where
+--     coe := by
+--       -- exists rule.captureEmbed
+--       sorry
+
+end Rule
